stack_args now synchronised

pcuic/theories/PCUICSafeConversion.v
@@ -2019,44 +2019,26 @@ Section Conversion.
     symmetry. assumption.
   Qed.
 
-  (* Definition stack_args (t : term) (π : stack) : list (term * stack) := *)
-  (*   let '(args, ρ) := decompose_stack π in *)
-  (*   fold_left (fun l u => (u, coApp ? ρ+++?)) args []. *)
-
-  Fixpoint stack_args (t : term) (π : stack) {struct π} : list (term * stack) :=
-    match π with
-    | App u ρ => (u, coApp t ρ) :: stack_args (tApp t u) ρ
-    | _ => []
-    end.
-
-  Equations stack_args_w Γ (t : term) (π : stack) (h : wtp Γ t π)
-    : list ({ x : term * stack | wtp Γ (fst x) (snd x) }) :=
-    stack_args_w Γ t (App u ρ) h :=
-      (exist (u, coApp t ρ) h) :: stack_args_w Γ (tApp t u) ρ h ;
-    stack_args_w Γ t ρ h := [].
-
-  (* Fixpoint stack_args_w (t : term) (π : stack) {struct π} : list (wterm * stack) := *)
-  (*   match π with *)
-  (*   | App u ρ => (u, coApp t ρ) :: stack_args (tApp t u) ρ *)
-  (*   | _ => [] *)
-  (*   end. *)
+  Equations stack_args Γ (t1 t2 : term) (π1 π2 : stack) (h2 : wtp Γ t2 π2)
+    : list (term * stack * { x : term * stack | wtp Γ (fst x) (snd x) }) :=
+    stack_args Γ t1 t2 (App u1 ρ1) (App u2 ρ2) h2 :=
+      (u1, coApp t1 ρ1, exist (u2, coApp t2 ρ2) h2)
+      :: stack_args Γ (tApp t1 u1) (tApp t2 u2) ρ1 ρ2 h2 ;
+    stack_args Γ t1 t2 π1 π2 h2 := [].
 
   Lemma foo :
     forall Γ t π1 π2 h2,
-      Forall2 (fun '(u1, ρ1) '(exist (u2, ρ2) h) =>
+      Forall (fun '(u1, ρ1, exist (u2, ρ2) h) =>
         R (mkpack (Reduction u2) Γ u1 ρ1 ρ2 h)
           (mkpack Args Γ t π1 π2 h2)
-      ) (stack_args t π1) (stack_args_w Γ t π2 h2).
+      ) (stack_args Γ t t π1 π2 h2).
   Proof.
     simpl. intros Γ t π1 π2 h2.
-    revert Γ t π2 h2.
-    induction π1 ; intros Γ u π2 h2.
-    - simpl. funelim (stack_args_w Γ u π2 h2).
-      all: try solve [ constructor ].
-      (* Maybe do it both at the same time. *)
-(*       econstructor. *)
-
-(* simp stack_args_w. *)
+    funelim (stack_args Γ t t π1 π2 h2).
+    all: try solve [ constructor ].
+    econstructor.
+    - unshelve eapply R_positionR.
+      + simpl.
 
 
   Abort.
